theories/Constr/CMapPartialOrder.v
@@ -1,4 +1,4 @@
-Require Import CSet CMap CMapDomain Infra.PartialOrder Infra.OptionR.
+Require Import CSet CMap CMapDomain Infra.PartialOrder Infra.OptionPO.
 
 Set Implicit Arguments.
 
