theories/Infra/Lattice.v
@@ -8,7 +8,7 @@ Updated to accomodate non-extensional equalities
 
 Require Export Containers.OrderedType Setoid Coq.Classes.Morphisms Computable.
 Require Export Util Get MoreList PartialOrder.
-Require Import EqDec DecSolve List AllInRel.
+Require Import EqDec DecSolve List AllInRel OptionPO.
 
 Class JoinSemiLattice (A : Type) `{PartialOrder A} :=
   {
@@ -22,6 +22,9 @@ Class JoinSemiLattice (A : Type) `{PartialOrder A} :=
       join_respects_eq :> Proper (poEq ==> poEq ==> poEq) join;
       join_respects_le :> Proper (poLe ==> poLe ==> poLe) join
   }.
+
+
+Arguments join : simpl never.
 
 Lemma join_wellbehaved
   : forall A `{JoinSemiLattice A} x y, poEq x (join x y) <-> poLe y x.
@@ -62,6 +65,8 @@ Class LowerBounded (A : Type) `{PartialOrder A} :=
 
 Infix "⊔" := join (at level 70, no associativity).
 Notation "⊥" := bottom (at level 70, no associativity).
+
+Arguments bottom : simpl never.
 
 Instance pair_semilattice A B `{JoinSemiLattice A} `{JoinSemiLattice B}
   : JoinSemiLattice (A * B) := {
@@ -108,8 +113,6 @@ Proof.
   intros; econstructor.
 Defined.
 
-Require Import OptionR.
-
 Definition ojoin A join (x y:option A) :=
   match x, y with
   | x, None => x
@@ -121,8 +124,7 @@ Instance ojoin_poEq A `{JoinSemiLattice A}
   : Proper (poEq ==> poEq ==> poEq) (ojoin A join).
 Proof.
   unfold Proper, respectful.
-  intros ? ? EQ ? ? EQ'; inversion EQ; inversion EQ'; subst; simpl;
-    eauto using option_R.
+  intros ? ? EQ ? ? EQ'; inversion EQ; inversion EQ'; subst; simpl; eauto.
   econstructor. rewrite H1, H4. reflexivity.
 Qed.
 
@@ -146,7 +148,7 @@ Proof.
       econstructor; eauto using join_bound.
   - intros [a|] [b|]; simpl; econstructor; eauto using join_commutative.
   - intros [a1|] [b1|] [c1|]; simpl; econstructor; eauto using join_associative.
-  - intros [a|] [b|]; simpl; econstructor; eauto using fstNoneOrR, join_poLe.
+  - intros [a|] [b|]; simpl; econstructor; eauto using join_poLe.
 Defined.
 
 Lemma join_struct T `{JoinSemiLattice T} (a b a' b':T)
@@ -227,3 +229,14 @@ Ltac clear_join_false :=
   end.
 
 Smpl Add clear_join_false : inv_trivial.
+
+
+Lemma join_poLe_left (X : Type) (H : PartialOrder X) (H0 : JoinSemiLattice X)
+      (x y z : X)
+  : x ⊑ z -> y ⊑ z -> x ⊔ y ⊑ z.
+Proof.
+  intros.
+  rewrite H1, H2.
+  rewrite (join_idempotent _ z).
+  reflexivity.
+Qed.
