theories/Infra/OptionPO.v
@@ -1,0 +1,109 @@
+Require Import Util DecSolve Coq.Classes.RelationClasses.
+Require Import Infra.PartialOrder Terminating Option OptionR.
+
+
+Instance PartialOrder_option Dom `{PartialOrder Dom}
+: PartialOrder (option Dom) := {
+  poLe := option_R poLe;
+  poLe_dec := @option_R_dec _ _ poLe poLe_dec;
+  poEq := option_R poEq;
+  poEq_dec := @option_R_dec _ _ poEq poEq_dec;
+}.
+Proof.
+  - intros; inv H0; eauto using option_R, poLe_refl.
+Defined.
+
+
+Instance terminating_option Dom `{PO:PartialOrder Dom}
+  : Terminating Dom poLt
+    -> Terminating (option Dom) poLt.
+Proof.
+  intros. hnf; intros.
+  destruct x.
+  - specialize (H d).
+    general induction H.
+    econstructor; intros. inv H1; inv H2.
+    eapply H0; eauto using option_R.
+    split; eauto. intro. eapply H3; econstructor; eauto.
+  - econstructor; intros. inv H0.
+    exfalso. inv H1. eapply H2; reflexivity.
+Qed.
+
+Instance PartialOrder_option_fstNoneOrR Dom `{PartialOrder Dom}
+: PartialOrder (option Dom) := {
+  poLe := fstNoneOrR poLe;
+  poLe_dec := _;
+  poEq := option_R poEq;
+  poEq_dec := _;
+}.
+Proof.
+  - intros; inv H0; eauto using fstNoneOrR, poLe_refl.
+Defined.
+
+Lemma poLe_opt_inv T H a b
+  : @poLe (option T) (@PartialOrder_option_fstNoneOrR T H)
+          (@Some T a) (@Some T b)
+    -> poLe a b.
+Proof.
+  inversion 1; eauto.
+Qed.
+
+Smpl Add
+     match goal with
+     | [ H : @poLe (option ?T) (@PartialOrder_option_fstNoneOrR ?T ?H')
+                   ?A (@Some ?T ?b) |- _ ] =>
+       eapply (@poLe_opt_inv T H') in H
+     | [ H : @poLe (option ?T) (@PartialOrder_option_fstNoneOrR ?T ?H')
+                   (@Some ?T ?a) None |- _ ] =>
+       exfalso; inv H
+     | [ H : @poLe (option ?T) (@PartialOrder_option_fstNoneOrR ?T ?H')
+                   None _ |- _ ] => clear H
+     end : inv_trivial.
+
+Lemma poEq_None_inv (T : Type) (H : PartialOrder T) a
+  : a ≣ None -> a = None.
+Proof.
+  intros. invc H0. reflexivity.
+Qed.
+
+Smpl Add
+     match goal with
+     | [ H : ?Y ≣ ⎣⎦ |- _ ] => eapply poEq_None_inv in H; try subst Y
+     | [ H : ⎣⎦ ≣ ?Y |- _ ] => symmetry in H; eapply poEq_None_inv in H; try subst Y
+     end : inv_trivial.
+
+Lemma poEq_Some_inv (T : Type) (H : PartialOrder T) a b
+  : a ≣ Some b -> exists a', a = Some a' /\ poEq a' b.
+Proof.
+  intros. invc H0. eauto.
+Qed.
+
+Smpl Add
+     match goal with
+     | [ H : ?Y ≣ Some _ |- _ ] => eapply poEq_Some_inv in H;
+                                   destruct H as [? [? H]]; try subst Y
+     | [ H : Some _ ≣ ?Y |- _ ] => symmetry in H; eapply poEq_Some_inv in H;
+                                   destruct H as [? [? H]]; try subst Y
+     end : inv_trivial.
+
+Lemma poLe_option_None X `{PartialOrder X} (x:option X)
+  :  None ⊑ x.
+Proof.
+  econstructor.
+Qed.
+
+Hint Resolve poLe_option_None.
+
+Lemma poLe_Some_struct A `{PartialOrder A} (a b : A)
+  : poLe a b
+    -> poLe (Some a) (Some b).
+Proof.
+  econstructor; eauto.
+Qed.
+
+Hint Resolve poLe_Some_struct.
+
+Smpl Add match goal with
+         | [ H : poLe _ None |- _ ] => invc H
+         | [ H : ⎣ ?x ⎦ <> ⎣ ?x ⎦ |- _ ] => exfalso; apply H; reflexivity
+         end : inv_trivial.
