theories/Infra/OptionR.v
@@ -1,5 +1,5 @@
 Require Import Util DecSolve Coq.Classes.RelationClasses.
-Require Import Infra.PartialOrder Terminating Option.
+Require Import Option.
 
 Set Implicit Arguments.
 
@@ -8,7 +8,6 @@ Definition mapOption A B (f:A -> B) (o:option A) : option B :=
   | Some a => Some (f a)
   | None => None
   end.
-
 
 Inductive option_R A B (R: A -> B -> Prop) : option A -> option B -> Prop :=
 | option_R_None : option_R R None None
@@ -55,33 +54,6 @@ Proof.
   decide (R a b); dec_solve.
 Defined.
 
-Instance PartialOrder_option Dom `{PartialOrder Dom}
-: PartialOrder (option Dom) := {
-  poLe := option_R poLe;
-  poLe_dec := @option_R_dec _ _ poLe poLe_dec;
-  poEq := option_R poEq;
-  poEq_dec := @option_R_dec _ _ poEq poEq_dec;
-}.
-Proof.
-  - intros; inv H0; eauto using option_R, poLe_refl.
-Defined.
-
-
-Instance terminating_option Dom `{PO:PartialOrder Dom}
-  : Terminating Dom poLt
-    -> Terminating (option Dom) poLt.
-Proof.
-  intros. hnf; intros.
-  destruct x.
-  - specialize (H d).
-    general induction H.
-    econstructor; intros. inv H1; inv H2.
-    eapply H0; eauto using option_R.
-    split; eauto. intro. eapply H3; econstructor; eauto.
-  - econstructor; intros. inv H0.
-    exfalso. inv H1. eapply H2; reflexivity.
-Qed.
-
 Inductive fstNoneOrR (X Y:Type) (R:X->Y->Prop)
   : option X -> option Y -> Prop :=
 | fstNone (x:option Y) : fstNoneOrR R None x
@@ -122,37 +94,6 @@ Proof.
   decide (R a b); dec_solve.
 Defined.
 
-Instance PartialOrder_option_fstNoneOrR Dom `{PartialOrder Dom}
-: PartialOrder (option Dom) := {
-  poLe := fstNoneOrR poLe;
-  poLe_dec := _;
-  poEq := option_R poEq;
-  poEq_dec := _;
-}.
-Proof.
-  - intros; inv H0; eauto using fstNoneOrR, poLe_refl.
-Defined.
-
-Lemma poLe_opt_inv T H a b
-  : @poLe (option T) (@PartialOrder_option_fstNoneOrR T H)
-          (@Some T a) (@Some T b)
-    -> poLe a b.
-Proof.
-  inversion 1; eauto.
-Qed.
-
-Smpl Add
-     match goal with
-     | [ H : @poLe (option ?T) (@PartialOrder_option_fstNoneOrR ?T ?H')
-                   ?A (@Some ?T ?b) |- _ ] =>
-       eapply (@poLe_opt_inv T H') in H
-     | [ H : @poLe (option ?T) (@PartialOrder_option_fstNoneOrR ?T ?H')
-                   (@Some ?T ?a) None |- _ ] =>
-       exfalso; inv H
-     | [ H : @poLe (option ?T) (@PartialOrder_option_fstNoneOrR ?T ?H')
-                   None _ |- _ ] => clear H
-     end : inv_trivial.
-
 
 Inductive ifFstR {X Y} (R:X -> Y -> Prop) : option X -> Y -> Prop :=
   | IfFstR_None y : ifFstR R None y
@@ -174,52 +115,3 @@ Smpl Add 100
      | [ H : @ifSndR _ _ _ _ ?B |- _ ] =>
        is_constructor_app B; invc H
      end : inv_trivial.
-
-
-Lemma poEq_None_inv (T : Type) (H : PartialOrder T) a
-  : a ≣ None -> a = None.
-Proof.
-  intros. invc H0. reflexivity.
-Qed.
-
-Smpl Add
-     match goal with
-     | [ H : ?Y ≣ ⎣⎦ |- _ ] => eapply poEq_None_inv in H; try subst Y
-     | [ H : ⎣⎦ ≣ ?Y |- _ ] => symmetry in H; eapply poEq_None_inv in H; try subst Y
-     end : inv_trivial.
-
-Lemma poEq_Some_inv (T : Type) (H : PartialOrder T) a b
-  : a ≣ Some b -> exists a', a = Some a' /\ poEq a' b.
-Proof.
-  intros. invc H0. eauto.
-Qed.
-
-Smpl Add
-     match goal with
-     | [ H : ?Y ≣ Some _ |- _ ] => eapply poEq_Some_inv in H;
-                                   destruct H as [? [? H]]; try subst Y
-     | [ H : Some _ ≣ ?Y |- _ ] => symmetry in H; eapply poEq_Some_inv in H;
-                                   destruct H as [? [? H]]; try subst Y
-     end : inv_trivial.
-
-Lemma poLe_option_None X `{PartialOrder X} (x:option X)
-  :  None ⊑ x.
-Proof.
-  econstructor.
-Qed.
-
-Hint Resolve poLe_option_None.
-
-Lemma poLe_Some_struct A `{PartialOrder A} (a b : A)
-  : poLe a b
-    -> poLe (Some a) (Some b).
-Proof.
-  econstructor; eauto.
-Qed.
-
-Hint Resolve poLe_Some_struct.
-
-Smpl Add match goal with
-         | [ H : poLe _ None |- _ ] => invc H
-         | [ H : ⎣ ?x ⎦ <> ⎣ ?x ⎦ |- _ ] => exfalso; apply H; reflexivity
-         end : inv_trivial.
