theories/ValueOpts/ConstantPropagationAnalysis.v
@@ -1,6 +1,6 @@
 Require Import CSet Le CMap CMapDomain CMapPartialOrder CMapJoinSemiLattice CMapTerminating.
 
-Require Import Plus Util AllInRel CSet OptionR.
+Require Import Plus Util AllInRel CSet OptionPO.
 Require Import Val Var Env IL Annotation Infra.Lattice DecSolve.
 Require Import Analysis.Analysis AnalysisForwardSSA ValueOpts.ConstantPropagation.
 
